Updated Dblist_proof.v

cfml/examples/Dblist/Dblist_proof.v
@@ -4,13 +4,17 @@ From CFML Require Import Stdlib.
 From EXAMPLES Require Import Dblist_ml.
 From TLC Require Import LibListZ.
 
-Definition Node A `{EA: Enc A} (v: A) (n p c: node_ A) : hprop :=
+Definition Node A `{EA: Enc A} (v: A) (n p c: loc) : hprop :=
   c ~~~> `{ data' := v; next' := n; prev' := p }.
 
-Lemma Node_open_close : forall A {EA: Enc A} (c: node_ A) (v: A) (n p: node_ A),
+Lemma Node_open_close : forall A {EA: Enc A} (c: loc) (v: A) (n p: loc),
   c ~> Node v n p
 = c ~~~> `{ data' := v; next' := n; prev' := p }.
 Proof using. auto. Qed.
+
+Lemma Node_affine : forall A {EA: Enc A} (c: loc) (v: A) (n p: loc),
+  haffine (c ~> Node v n p).
+Proof using. intros. xunfold Node. xaffine. Qed.
 
 (** A segment of a doubly-linked list. *)
 (* Arguments:
@@ -23,32 +27,44 @@ Proof using. auto. Qed.
               This is actually the address stored in the [prev] field of
               the [from] pointer.
 *)
-Fixpoint NodeSeg A `{EA: Enc A} (L: list A) (to last first from: node_ A) : hprop :=
+Fixpoint NodeSeg A `{EA: Enc A} (L: list A) (to last first from: loc) : hprop :=
   match L with
   | nil => \[to = from] \* \[last = first]
   | x :: L' =>
-      \exists (n: node_ A), (from ~> Node x n first) \* (n ~> NodeSeg L' to last from)
+      \exists (n: loc), (from ~> Node x n first) \* (n ~> NodeSeg L' to last from)
   end.
 
+Lemma NodeSeg_if : forall A {EA: Enc A} (from: loc) (L: list A) (to last first: loc),
+  from ~> NodeSeg L to last first =
+    If from = to then \[L = nil]
+    else \exists x L', \[L = x :: L'].
+Admitted.
+
+Lemma NodeSeg_if2 : forall A {EA: Enc A} (from: loc) (L: list A) (to last first: loc),
+  from ~> NodeSeg L to last first =
+    If last = first then \[L = nil] \* from ~> NodeSeg (@nil A) to last first
+    else \exists x L', \[L = x :: L'] \* from ~> NodeSeg (x::L') to last first.
+Admitted.
+
 Lemma NodeSegBackward :
-  forall A {EA: Enc A} (from: node_ A) (v: A) (L: list A) (to last first: node_ A),
+  forall A {EA: Enc A} (from: loc) (v: A) (L: list A) (to last first: loc),
     from ~> NodeSeg (L&v) to last first
- ==> \exists (p: node_ A),
+ ==> \exists (p: loc),
    from ~> NodeSeg L last p first \* last ~> Node v to p.
 Admitted.
 
 Fixpoint NodeSeg_backward
-  A `{EA: Enc A} (L: list A) (to first from last: node_ A) : hprop :=
+  A `{EA: Enc A} (L: list A) (to first from last: loc) : hprop :=
   match L with
   | nil => \[to = from] \* \[last = first]
   | x :: L' =>
-      \exists (p: node_ A),
+      \exists (p: loc),
           (last ~> Node x to p) \*
           (p ~> NodeSeg_backward L' last first from)
   end.
 
 (* Lemma NodeSeg_open_close : *)
-(*   forall A {EA: Enc A} (c: node_ A) (v: A) (L: list A) (to last first n from: node_ A), *)
+(*   forall A {EA: Enc A} (c: loc) (v: A) (L: list A) (to last first n from: loc), *)
 (*   (from ~> Node v n first) \* (n ~> NodeSeg L to last from) *)
 (* = from ~> NodeSeg (v::L) to last first. *)
 (* Proof using. *)
@@ -56,17 +72,17 @@ Fixpoint NodeSeg_backward
 (*   xsimpl* *)
 
 Lemma NodeSeg_cons :
-  forall A {EA: Enc A} (from: node_ A) (v: A) (L: list A) (to last first: node_ A),
+  forall A {EA: Enc A} (from: loc) (v: A) (L: list A) (to last first: loc),
     from ~> NodeSeg (v::L) to last first
-  = \exists (n: node_ A), (from ~> Node v n first) \* (n ~> NodeSeg L to last from).
+  = \exists (n: loc), (from ~> Node v n first) \* (n ~> NodeSeg L to last from).
 Proof using. eauto. Qed.
 
-Lemma NodeSeg_nil : forall A (EA: Enc A) (from to last first: node_ A),
-  from ~> NodeSeg nil to last first
+Lemma NodeSeg_nil : forall A (EA: Enc A) (from to last first: loc),
+  from ~> NodeSeg (@nil A) to last first
 = \[to = from] \* \[last = first].
 Proof using. auto. Qed.
 
-Lemma NodeSeg_of_Node : forall A (EA: Enc A) (v: A) (c: node_ A),
+Lemma NodeSeg_of_Node : forall A (EA: Enc A) (v: A) (c: loc),
    c ~> Node v c c
 ==> c ~> NodeSeg (v::nil) c c c.
 Proof using.
@@ -76,17 +92,26 @@ Proof using.
   xsimpl*.
 Qed.
 
-Lemma node_of_NodeSeg : forall A (EA: Enc A) (v: A) (c: node_ A),
+Lemma node_of_NodeSeg : forall A (EA: Enc A) (v: A) (c: loc),
    c ~> NodeSeg (v::nil) c c c
 ==> c ~> Node v c c.
 Proof using.
   intros. xchange NodeSeg_cons ;=> n. xchanges* NodeSeg_nil.
 Qed.
 
+Lemma NodeSeg_affine : forall A {EA: Enc A} (from: loc) (L: list A) (to last first: loc),
+  haffine (from ~> NodeSeg L to last first).
+Proof using.
+  intros. gen from to last first. induction L as [| x L']; intros.
+  { xunfold NodeSeg. xaffine. }
+  { xunfold NodeSeg. xaffine.
+    applys Node_affine. }
+Qed.
+
 Lemma NodeSeg_forward_backward:
-  forall A {EA: Enc A} (x: A) (L: list A) (to last first from: node_ A),
+  forall A {EA: Enc A} (x: A) (L: list A) (to last first from: loc),
   from ~> NodeSeg (x :: L) to last first
-= last ~> NodeSeg_backward (x :: rev L) to first from.
+= last ~> NodeSeg_backward (rev L & x) to first from.
 Proof using.
   intros A EA L.
   (* induction_wf IH : list_sub L. destruct L as [| x L']; intros. *)
@@ -98,7 +123,7 @@ Admitted.
 Definition InnerNode A `{EA: Enc A} (L: list A) (p: innerNode_ A) : hprop :=
   match L with
   | nil => \[p = Nil]
-  | _ => \exists (c q: node_ A), \[p = Cons c] \* c ~> NodeSeg L c q q
+  | _ => \exists (c q: loc), \[p = Cons c] \* c ~> NodeSeg L c q q
   end.
 
 Lemma InnerNode_Nil : forall A (EA: Enc A) L,
@@ -117,10 +142,10 @@ Proof using. intros A EA. xunfolds* InnerNode. Qed.
 
 Lemma InnerNode_cons : forall A (EA: Enc A) (v: A) (L: list A) (p: innerNode_ A),
   p ~> InnerNode (v::L)
-= \exists (c q: node_ A), \[p = Cons c] \* c ~> NodeSeg (v::L) c q q.
+= \exists (c q: loc), \[p = Cons c] \* c ~> NodeSeg (v::L) c q q.
 Proof using. intros A EA v L p. auto. Qed.
 
-Lemma InnerNode_of_NodeSeg : forall A (EA: Enc A) (v: A) (L: list A) (c q: node_ A),
+Lemma InnerNode_of_NodeSeg : forall A (EA: Enc A) (v: A) (L: list A) (c q: loc),
   c ~> NodeSeg (v::L) c q q
 ==> Cons c ~> InnerNode (v::L).
 Proof using. intros. xunfolds* InnerNode. Qed.
@@ -140,7 +165,7 @@ Proof using.
     { xpull*; xsimpl*. } }
 Qed.
 
-Definition DbList A `{EA: Enc A} (L: list A) (l: loc) : hprop :=
+Definition Dblist A `{EA: Enc A} (L: list A) (l: loc) : hprop :=
   \exists (p q: innerNode_ A),
       (l ~~~> `{ head' := p; tail' := q; length' := length L })
         (* Mário: maybe I can keep this but move it down *)
@@ -151,9 +176,9 @@ Definition DbList A `{EA: Enc A} (L: list A) (l: loc) : hprop :=
          \exists x L' h t, \[L = x :: L'] \* \[p = Cons h] \* \[q = Cons t]
                         \* (h ~> NodeSeg L h t t)).
 
-Lemma Dblist_If : forall A (EA: Enc A) (L: list A) (l: loc),
-    l ~> DbList L =
-      \exists p q,
+Lemma Dblist_If : forall A {EA: Enc A} (L: list A) (l: loc),
+    l ~> Dblist L =
+      \exists (p q : innerNode_ A),
           (l ~~~> `{ head' := p; tail' := q; length' := length L }) \*
             (If q = Nil then
                \[L = nil] \* \[p = Nil]
@@ -162,8 +187,8 @@ Lemma Dblist_If : forall A (EA: Enc A) (L: list A) (l: loc),
 Admitted.
 
 Lemma Dblist_If_head : forall A (EA: Enc A) (L: list A) (l: loc),
-    l ~> DbList L =
-      \exists p q,
+    l ~> Dblist L =
+      \exists (p q : innerNode_ A),
           (l ~~~> `{ head' := p; tail' := q; length' := length L }) \*
             (If p = Nil then
                \[L = nil] \* \[q = Nil]
@@ -171,10 +196,17 @@ Lemma Dblist_If_head : forall A (EA: Enc A) (L: list A) (l: loc),
                                  \[q = Cons t] \* (h ~> NodeSeg L h t t)).
 Admitted.
 
+Lemma Dblist_nil : forall (l: loc) A `{EA: Enc A},
+  l ~> Dblist (@nil A) =
+  \exists (h t: innerNode_ A),
+  (l ~~~> `{ head' := h; tail' := t; length' := 0 }) \* \[h = Nil] \* \[t = Nil].
+Admitted.
+
+
 Section Ops.
   Context A {EA: Enc A}.
   Implicit Types L: list A.
-  Implicit Types c: node_ A.
+  Implicit Types c: loc.
   Implicit Types t: loc.
 
   Lemma Triple_create_node: forall (v: A),
@@ -182,7 +214,7 @@ Section Ops.
         PRE \[]
         POST (fun c => c ~> Node v c c).
   Proof using.
-    intros v. xcf. xapp ;=> c. xpull. xvals.
+    intros v. xcf. xapp ;=> c. xvals.
   Qed.
 
   Lemma Triple_create_node_seg: forall (v: A),
@@ -199,16 +231,16 @@ Section Ops.
   Lemma Triple_create :
     SPEC (create tt)
       PRE \[]
-      POST (fun t => t ~> DbList (@nil A)).
+      POST (fun t => t ~> Dblist (@nil A)).
   Proof using.
-    xcf. xapp* ;=> t. xunfolds* DbList.
+    xcf. xapp* ;=> t. xunfolds* Dblist.
     case_if. xsimpl*.
     (* xunfold InnerNode; xsimpl*. *)
     (* case_if. xsimpl. auto. auto. *)
   Qed.
 
   Lemma Triple_insert_after_node:
-    forall (L: list A) (x: A) (c n: node_ A) (to last first: node_ A),
+    forall (L: list A) (x: A) (c n: loc) (to last first: loc),
       SPEC (node_insert_after c n)
         PRE (n ~> Node x n n \* c ~> NodeSeg L to last first)
         POSTUNIT (n ~> NodeSeg L to last c ).
@@ -217,15 +249,15 @@ Proof using. intros. xcf. Admitted.
 
   Lemma Triple_push_end : forall L (v: A) t,
       SPEC (insert_back t v)
-        PRE (t ~> DbList L)
-        POSTUNIT (t ~> DbList (L & v)).
+        PRE (t ~> Dblist L)
+        POSTUNIT (t ~> Dblist (L & v)).
   Proof using.
     intros L v t. xcf.
     xchanges* Dblist_If ;=>.
     xapp Triple_create_node ;=> c.
     xapp. case_if; xpull ;=>; xmatch.
     { xapp. xapp. xapp. xapp. subst L.
-      xunfold DbList. case_if. rew_list*.
+      xunfold Dblist. case_if. rew_list*.
       xsimpl*.
       (* Mário: the following tactic does [xchange] + [xsimpl].
          [xchanges] = [xchange; xsimpl] *)
@@ -233,7 +265,7 @@ Proof using. intros. xcf. Admitted.
     (* Mário: the above finishes the case of the empty list *)
 
 
-    (* xunfold DbList. xpull* ;=> p. intros. *)
+    (* xunfold Dblist. xpull* ;=> p. intros. *)
     (* xchanges* InnerNode_If. case_if. *)
     (* { xpull* ;=> ->. xapp. xmatch. *)
     (*   xapp. xapp. xapp. xapp. case_if. *)
@@ -297,11 +329,26 @@ Proof using. intros. xcf. Admitted.
                     PRE (I L1)
                     POSTUNIT (I (L1 & x))) ->
       L = L1 ++ L2 ->
+      L2 <> nil ->
       SPEC (iter_left_aux f n e)
         PRE  (n ~> NodeSeg L2 h e p\* I L1)
         POSTUNIT (n ~> NodeSeg L2 h e p \* I L).
-  Proof using. (* introv SpecF. xcf. xunfold DbList. xpull. intros. xapp. xchange Dblist_If. *)
-  Admitted.
+  Proof using.
+    introv Specf. gen L1 n p.
+    induction_wf IH : list_sub L2.
+    xcf. destruct L2 as [| x2 L2']; tryfalse.
+    xchange NodeSeg_cons ;=>. xchange Node_open_close.
+    xunfold NodeSeg at 2.
+    xapp. xapp (Specf x2 L1 L2'); eauto.
+    xapp. xif; =>.
+    { xchange NodeSeg_if2. case_if. xpull*; =>.
+      subst L2'; rew_list*. xchange NodeSeg_cons ;=>.
+      xapp. xchange <- NodeSeg_cons. xapp; rew_list*; eauto.
+      intros false; false.
+      xsimpl*. xchanges <- Node_open_close. }
+    { xchange NodeSeg_if2. case_if. xpull*; => ->.
+      subst. xchanges <- Node_open_close. xvals. }
+  Qed.
 
   Lemma Triple_iter_left : forall (I: list A -> hprop) L (f: val) t,
       (forall x L1 L2, L = L1 ++ x :: L2 ->
@@ -309,19 +356,73 @@ Proof using. intros. xcf. Admitted.
           PRE (I L1)
           POSTUNIT (I (L1 & x))) ->
       SPEC (iter_left f t)
-        PRE (t ~> DbList L \* I nil)
-        POSTUNIT (t ~> DbList L \* I L).
+        PRE (t ~> Dblist L \* I nil)
+        POSTUNIT (t ~> Dblist L \* I L).
   Proof using.
     introv Specf.
     xcf. xchange* Dblist_If_head ;=>. xapp. case_if; xpull ;=>; xmatch.
-    { xval. subst L. subst x0. xsimpl*. xunfold DbList.
+    { xval. subst L. subst x0. xsimpl*. xunfold Dblist.
       case_if. xsimpl*. }
     { inversion TEMP; subst.
       xchange NodeSeg_cons ;=> .
       xapp. xmatch.
       xchange <- NodeSeg_cons.
       xapp (@Triple_iter_left_aux f I (x1::x2) nil); rew_list*.
-      xunfolds DbList; rew_list*. case_if. xsimpl*. }
+      { intros false; false. }
+      xunfolds Dblist; rew_list*. case_if. xsimpl*. }
     Qed.
+
+  Lemma Triple_fold_left_aux :
+    forall {B} (f: val) (I : B -> list A -> hprop) (L L1 L2: list A) (acc: B) n e h p,
+      (forall acc x L1 L2, L = L1 ++ x :: L2 ->
+                  SPEC (f acc x)
+                    PRE (I acc L1)
+                    POST (fun accu => I accu (L1 & x))) ->
+      L = L1 ++ L2 ->
+      SPEC (fold_left_aux f acc n e)
+        PRE (n ~> NodeSeg L2 h e p \* I acc L1)
+        POST (fun accu => n ~> NodeSeg L2 h e p \* I accu L).
+  Proof using. Admitted.
+
+  Lemma Triple_fold_left : forall {B} (I: B -> list A -> hprop) L (f: val) t (acc: B),
+      (forall acc x L1 L2, L = L1 ++ x :: L2 ->
+        SPEC (f acc x)
+          PRE (I acc L1)
+          POST (fun accu => I accu (L1 & x))) ->
+      SPEC (Dblist_ml.fold_left f acc t)
+        PRE (t ~> Dblist L \* I acc nil)
+        POST (fun accu => t ~> Dblist L \* I accu L).
+  Proof using.
+    introv Specf. xcf. xchange* Dblist_If_head ;=>.
+    xapp. case_if; xpull ;=>; xmatch.
+    { xval. subst L. subst x0. xsimpl*. xunfold Dblist.
+      case_if. xsimpl*. }
+    { inversion TEMP; subst.
+      xchange NodeSeg_cons ;=> .
+      xapp. xmatch.
+      xchange <- NodeSeg_cons.
+      xapp (@Triple_fold_left_aux B f I (x1::x2) nil); rew_list*.
+      xunfolds Dblist; rew_list*. case_if. xsimpl*.
+    }
+  Qed.
+
+  Lemma Triple_clear : forall (p: loc) (L: list A) (h t: innerNode_ A),
+    SPEC (clear p)
+      PRE (p ~~~> `{ head' := h; tail' := t; length' := length L })
+      POSTUNIT (p ~> Dblist (@nil A)).
+  Proof using.
+    intros. xcf. xapp. xapp. xapp. xchanges* <- Dblist_nil.
+  Qed.
+
+  Lemma Triple_clear_alt : forall (p: loc) (L: list A) (h t: innerNode_ A),
+    SPEC (clear p)
+      PRE (p ~> Dblist L)
+      POSTUNIT (p ~> Dblist (@nil A)).
+  Proof using.
+    intros. xcf. xunfold Dblist; xpull ;=>. xapp. case_if; xpull ;=>.
+    { xapp. xapp. case_if. xsimpl*. }
+    { xapp. xapp. case_if. xsimpl*. applys NodeSeg_affine. }
+  Qed.
+
 
 End Ops.
